pcuic/theories/PCUICValidity.v
@@ -1,33 +1,81 @@
 From Coq Require Import Bool String List Program BinPos Compare_dec Omega.
 From Template Require Import utils.
-From PCUIC Require Import PCUICAst PCUICAstUtils PCUICInduction PCUICLiftSubst PCUICTyping PCUICWeakening.
+From PCUIC Require Import PCUICAst PCUICAstUtils PCUICInduction PCUICLiftSubst PCUICTyping. (* PCUICWeakening. *)
+Require Import ssreflect.
 Existing Instance config.default_checker_flags.
 Lemma type_local_env_isdecl Σ n Γ :
-  forall isdecl : n < #|Γ|, All_local_env typing Σ Γ ->
+  forall isdecl : n < #|Γ|, All_local_env (lift_typing typing) Σ Γ ->
   { Γ' : _ & { Γ'' : _ &
                     { _ : type_local_decl Σ Γ'' (safe_nth Γ (exist _ n isdecl)) &
                     Γ = Γ' ++ Γ'' /\ #|Γ'| = S n } } }.
 Proof. Admitted.
 
-Theorem validity : env_prop (fun Σ Γ t T => wf_local Σ Γ -> isType_or_Sort Σ Γ T).
+Definition property :=
+  forall (Σ : global_context) (Γ : context),
+    All_local_env (lift_typing typing) Σ Γ -> forall t T : term, typing Σ Γ t T -> Type.
+
+(* Definition lookup_wf_local Σ Γ (wfΓ : wf_local Σ Γ) (n : nat | n < #|Γ|) : *)
+(*   { wf : wf_local Σ (skipn (S n) Γ) & *)
+
+(*          let decl := safe_nth Γ n in *)
+(*          typing Σ (skipn (S n) Γ) *)
+(*          Q \Sigma \Gamma *)
+
+
+
+(* Definition on_wf_local_decl Σ Γ (wfΓ : wf_local Σ Γ) (P : property) d := *)
+(*   match d.(decl_body) with *)
+(*   | Some b => Q Σ Γ b (Some d.(decl_type)) *)
+(*   | None => P Σ Γ d.(decl_type) None *)
+(*   end. *)
+
+(* Lemma nth_error_All_local_env_over {P Q Σ Γ n} (isdecl : n < #|Γ|) (wfΓ : All_local_env P Σ Γ) : *)
+(*   All_local_env_over P Q Σ Γ wfΓ -> *)
+(*   on_some (on_local_decl (fun Σ Γ t T => P Σ (skipn (S n) Γ)) (nth_error Γ n)). *)
+(* Proof. *)
+(*   induction 1 in n, isdecl |- *. red; simpl. *)
+(*   - destruct n; simpl; inv isdecl. *)
+(*   - destruct n. red; simpl. red. simpl. apply t0. *)
+(*     simpl. apply IHX. simpl in isdecl. lia. *)
+(*   - destruct n. auto. *)
+(*     apply IHX. simpl in *. lia. *)
+(* Qed. *)
+
+(* Require Import LibHypsNaming. *)
+From Equations Require Import Equations.
+Theorem validity :
+  env_prop (fun Σ Γ t T => isType_or_Sort Σ Γ T).
 Proof.
-  apply typing_ind_env; intros.
+  apply typing_ind_env; intros; rename_all_hyps.
 
-  - pose proof H as H0.
-    eapply (All_local_env_lookup X) in H.
-    red in H |- *. destruct decl as [na [b|] ty]. cbn -[skipn] in *.
-    forward H by auto with wf.
-    destruct H. left; destruct ty; simpl in i; depelim i. exact I.
-    right. destruct i as [u Hu].
-    exists u.
+  - induction X. destruct n; discriminate.
+    simpl in *. destruct tu as [u Hu]. simpl in *.
+    destruct n. simpl in *. noconf heq_nth_error.
+    simpl. red. right. exists u. admit.
 
 
+    destruct decl as [na' [b|] ty].
+    destruct decl as [na [b|] ty]; cbn -[skipn] in *.
+    + destruct Hd as [Hty|[u Hu]].
+      ++ left; destruct ty; simpl in *; now destruct Hty.
+      ++ right. exists u.
+         (* epose proof (weakening _ _ (firstn (S n) Γ) _ _ _ _ Hu) as Hw. *)
+         (* rewrite [_ ,,, _]firstn_skipn in Hw. *)
+         (* rewrite firstn_length_le in Hw. apply nth_error_Some_length in heq_nth_error. auto with arith. *)
+         (* apply Hw. *) admit.
+    + simpl in *. destruct Hd as [u [Hs|Hty]].
 
-    apply (type_local_env_isdecl _ _ _ H0) in X0. as [Γ' [Γ'' [H0 [-> <-]]]].
-    destruct safe_nth. simpl in *.
-    red in H0. simpl in H0. destruct decl_body. admit.
-    destruct H0. exists x. 
-    now refine (weakening _ _ _ _ _ _ _ t). 
+    pose proof (All_local_env_lookup HΓ0 heq_nth_error) as Hd.
+    red in Hd |- *. destruct decl as [na [b|] ty]; cbn -[skipn] in *.
+    + destruct Hd as [Hty|[u Hu]].
+      ++ left; destruct ty; simpl in *; now destruct Hty.
+      ++ right. exists u.
+         (* epose proof (weakening _ _ (firstn (S n) Γ) _ _ _ _ Hu) as Hw. *)
+         (* rewrite [_ ,,, _]firstn_skipn in Hw. *)
+         (* rewrite firstn_length_le in Hw. apply nth_error_Some_length in heq_nth_error. auto with arith. *)
+         (* apply Hw. *) admit.
+    + simpl in *. destruct Hd as [u [Hs|Hty]].
+
 
   - exists (succ_sort (succ_sort s)). constructor.
   - now exists s.
